examples/steel/Duplex.PCM.fsti
@@ -1,0 +1,67 @@
+module Duplex.PCM
+open Steel.Channel.Protocol
+open Steel.Memory
+open Steel.Effect
+
+let dprot' = protocol unit
+
+// Simplifying protocols for now
+let rec no_loop (p:protocol 'a) =
+  match p with
+  | Return _ -> True
+  | Msg _ a k -> (forall x. no_loop (k x))
+  | DoWhile _ _ -> False
+
+let dprot = p:dprot'{no_loop p}
+
+type party = | A | B
+
+let nl_protocol 'a = p:protocol 'a { no_loop p }
+let return (#a:_) (x:a) : nl_protocol a = Return x
+let done : dprot = return ()
+let send_msg a : nl_protocol a = Msg Send a return
+let recv_msg a : nl_protocol a = Msg Recv a return
+let rec bind #a #b (p:nl_protocol a) (q:(a -> nl_protocol b))
+  : nl_protocol b
+  = match p with
+    | Return v -> q v
+    | Msg tag c #a' k ->
+       let k : c -> nl_protocol b =
+        fun x -> bind (k x) q
+      in
+      Msg tag c k
+
+let step (p:dprot{more_msgs p})
+         (x:next_msg_t p)
+  : dprot
+  = Msg?.k (hnf p) x
+
+let is_send_next name (next:dprot) =
+  more next /\ tag_of next == (if name = A then Send else Recv)
+let is_recv_next name (next:dprot) =
+  more next /\ tag_of next == (if name = A then Recv else Send)
+
+type send_next_dprot_t (name:party) =
+  next:dprot{more next /\ tag_of next == (if name = A then Send else Recv)}
+
+type recv_next_dprot_t (name:party) =
+  next:dprot{more next /\ tag_of next == (if name = A then Recv else Send)}
+
+val ch : Type u#1
+
+val ep (name:party) (c:ch) (next:dprot) : slprop u#1
+
+val send (#name:party)
+         (#next:dprot)
+         (c:ch { is_send_next name next })
+         (x:msg_t next)
+  : SteelT unit
+      (ep name c next)
+      (fun _ -> ep name c (step next x))
+
+val recv (#name:party)
+         (#next:dprot)
+         (c:ch { is_recv_next name next })
+  : SteelT (msg_t next)
+      (ep name c next)
+      (fun x -> ep name c (step next x))
